SEARsettings.sml
@@ -1,4 +1,34 @@
 
+local
+fun delete'(set,mem) = HOLset.delete(set,mem) handle _ => set
+in
+fun filter_cont ct = 
+    HOLset.foldr 
+        (fn (ns,set) => 
+            case HOLset.find 
+                     (fn (vn,vs) => HOLset.member(fvs vs,ns)) set of 
+                SOME _ => delete'(set,ns)
+              | NONE => set) ct ct
+end
+
+fun ex2fsym fsym strl th = 
+    let val th' = spec_all th
+        val (ct,asl) = (cont th',ant th')
+        val (hyp,conc) = dest_imp (concl th')
+        val inputvars0 = filter_cont (cont th') 
+        val inputvars = List.foldr (fn (s,e) => HOLset.add(e,s)) essps 
+                                   (List.map (dest_var o (parse_term_with_cont ct)) strl)
+        val _ = HOLset.isSubset(inputvars0,inputvars) orelse 
+                raise simple_fail "there are necessary input variables missing"
+        val inputvl = List.map (parse_term_with_cont ct) strl
+        val ((n,s),b) = dest_exists conc
+        val _ = new_fun fsym (s,List.map dest_var inputvl)
+        val fterm = mk_fun fsym inputvl
+        val b' = substf ((n,s),fterm) b
+    in mk_thm (ct,asl,mk_imp hyp b')
+    end
+
+
 fun new_ax f = 
     let
         val _ = HOLset.equal(fvf f,essps) orelse
@@ -18,6 +48,7 @@ fun mem_sort A = mk_sort "mem" [A]
 fun rel_sort A B = mk_sort "rel" [A,B]
 fun mk_set A = mk_var(A,set_sort)
 fun mk_rel R A B = mk_var(R,rel_sort A B)
+fun mk_mem a A = mk_var(a,mem_sort A)
 
 val _ = EqSorts := "rel" :: (!EqSorts)
 val _ = EqSorts := "mem" :: (!EqSorts)
@@ -82,12 +113,28 @@ fun AX1 (f:form) (a0 as (n1,s1),b0 as (n2,s2)) =
 
 (*Definition 2.1. A relation φ:A↬B is called a function from A to B if for any x∈A, there exists exactly one y∈B with φ(x,y).*)
 val _ = new_pred "isFun" [("R",rel_sort (mk_set "A") (mk_set "B"))]
+val _ = new_pred "isInj" [("R",rel_sort (mk_set "A") (mk_set "B"))]
+val _ = new_pred "isSurj" [("R",rel_sort (mk_set "A") (mk_set "B"))]
+val _ = new_pred "isBij" [("R",rel_sort (mk_set "A") (mk_set "B"))]
+
 val Fun_def = new_ax “!A B R:rel(A,B). isFun(R) <=> !x:mem(A). ?!y:mem(B). Holds(R,x,y)”
+
 
 val _ = new_fun "Eval" (mem_sort (mk_set "B"),[("R",rel_sort (mk_set "A") (mk_set "B")),
                         ("x",mem_sort (mk_set "A"))])
 
 val Eval_def = new_ax “!A B Fn:rel(A,B). isFun(Fn) ==>!x y. Holds(Fn,x,y) <=> y = Eval(Fn,x)”
+
+val Inj_def = new_ax “!A B R:rel(A,B). isInj(R) <=> !x1:mem(A) x2:mem(A) y:mem(B). Holds(R,x1,y) & Holds(R,x2,y) ==> x1 = x2”
+val Surj_def = new_ax “!A B R:rel(A,B). isSurj(R) <=> !y:mem(B).?x:mem(A). Holds(R,x,y)”
+
+val _ = new_pred "isTab" [("R",rel_sort (mk_set "A") (mk_set "B")),
+                          ("p",rel_sort (mk_set "TR") (mk_set "A")),
+                          ("q",rel_sort (mk_set "TR") (mk_set "B"))]
+
+val Tab_def = new_ax
+“!A B R TR p:TR->A q:TR->B.isTab(R,p,q) <=> 
+ (!x y. Holds(R,x,y) <=> ?r. Eval(p,r) = x & Eval(q,r) = y) & !r s. Eval(p,r) = Eval(p,s) & Eval(q,r) = Eval(q,s) ==> r = s”
 
 (*
 Axiom 2 (Tabulations): For any relation φ:A↬B, there exists a set |φ| and functions p:|φ|→A and q:|φ|→B such that: (1) for any x∈A and y∈B, we have φ(x,y) if and only if there exists r∈|φ| with p(r)=x and q(r)=y, and (2) for any r∈|φ| and s∈|φ|, if p(r)=p(s) and q(r)=q(s), then r=s.
@@ -103,10 +150,11 @@ val _ = new_fun "π2" (rel_sort (mk_set "TR") (mk_set "B"),[("R",rel_sort (mk_se
 (*how to let the ex2fsym function skip the TR and assign function symbols pi1 pi2?*)
 val AX2 = new_ax “!A B R:A->B.?TR p:TR->A q:TR->B. (!x y. Holds(R,x,y) <=> ?r. Eval(p,r) = x & Eval(q,r) = y) & !r s. Eval(p,r) = Eval(p,s) & Eval(q,r) = Eval(q,s) ==> r = s”
 
+(*
 Theorem 2.2. There exists a set ∅ which has no elements.
 
 Proof. By Axiom 0, there exists a set A. By Axiom 1, there exists a relation φ:A↬A such that φ(x,y) holds never. Using Axiom 2, let ∅ be a tabulation of φ.  ▮
-
+*)
 
 (*how can we just type the name once? for prove_store*)
 (*rw you idiot gives me  ~(~a'' = a'' & b = b)*)
@@ -159,11 +207,7 @@ val _ = new_fun "1" (set_sort,[])
 val ONE = mk_fun "1" []
 val _ = new_fun "star" (mem_sort ONE,[])
 
-val Thm_2_3_5 = proved_th $
-e0
-()
-(form_goal
- “!A.”)
+
 
 fun Rel2Pred P (ns as (n,s)) =
     let val onens = ("one0",mem_sort ONE)
@@ -177,7 +221,9 @@ e0
 (form_goal
 “!A R:1 -> A. ?B i:B->A. !a:mem(A).Holds(R,star,a) <=> ?b. a = Eval(i,b)”)
 
+(*
 Theorem 2.4. For any property P of elements of a set A, there exists a set B and an injective function i:B→A such that for a∈A, we have P(a) iff a=i(b) for some b∈B.
+*)
 
 fun uex_ex f = 
     let val th0 = iffLR $ uex_def f |> undisch
@@ -189,7 +235,8 @@ fun uex_ex f =
     in disch f th3
     end
 
-val P = “a:mem(A) = b”
+(*val P = “a:mem(A) = b”*)
+
 fun Thm_2_4 P (ns as (n,s)) = 
     let val l1 = Rel2Pred P ns
         val l1' = dimp_mp_l2r l1 (uex_def $ concl l1)
@@ -205,38 +252,525 @@ fun Thm_2_4 P (ns as (n,s)) =
     in exEed
     end
 
+(*
+Theorem 2.5. If |φ| and |φ|′ are two tabulations of the same relation φ:A↬B, then there is a bijection between |φ| and |φ|′.
+*)
 
-existsE l1' 
-rewr_rule[Thm_2_4_R_ver] (dimp_mp_l2r l1 (uex_def $ concl l1))
+val Thm_2_5 = proved_th $
+e0
+(cheat)
+(form_goal
+“!A B R:A->B T1 p1:T1->A q1:T1->B T2 p2:T2->A q2:T2->B.isTab(R,p1,q1) & isTab(R,p2,q2) ==> ?b:T1 ->T2.isBij(b)”)
+
 
 (*
-val ast1 =
-   aInfix
-    (aId "R", ":",
-     aApp
-      ("rel",
-       [aInfix
-         (aInfix (aId "A", ":", aApp ("set", [])), ":", aApp ("set", [])),
-        aInfix
-         (aInfix (aId "A", ":", aApp ("set", [])), ":", aApp ("set", []))])):
-   ast
+Corollary 2.6. If |S| and |S|′ are two tabulations of the same subset S⊆A, then there is a bijection between |S| and |S|′.
 
 
-local
-val lemma = AX1 “~(a:mem(A) = a)” (("a",mem_sort (mk_set "A")),("a",mem_sort (mk_set "A")))
-in
-val Thm_2_2 = proved_th $ val (ct,_,_) = cg $
+The composite of two relations φ:A↬B and ψ:B↬C is defined to be the relation ψφ:A↬C (also written ψ∘φ) such that ψφ(x,z) holds of x∈A and z∈C iff there is a y∈B with φ(x,y) and ψ(y,z). The identity relation idA:A↬A is defined by idA(x,y)⇔x=y.
+
+Theorem 2.7. Composition of relations is associative (χ(ψφ)=(χψ)φ), and identity relations are identities for composition (idB∘φ=φ=φ∘idA). The composite of functions is a function, and the identity relation is a function. The composite of bijections is a bijection, and a relation φ:A↬B is a bijection iff there is a relation ψ:B↬A such that ψφ=idA and φψ=idB.
+*)
+
+val _ = new_fun "o" (rel_sort (mk_set "A") (mk_set "C"),
+                     [("phi",rel_sort (mk_set "B") (mk_set "C")),
+                      ("psi",rel_sort (mk_set "A") (mk_set "B"))])
+
+(*AQ: phi still not parsable, too many phis of different versions.*)
+val o_def = new_ax 
+“!A B phi:A->B C psi:B->C a:mem(A) c:mem(C). 
+(?b. Holds(phi,a,b) & Holds(psi,b,c)) <=> Holds(psi o phi,a,c)”
+
+val _ = new_fun "id" (rel_sort (mk_set "A") (mk_set "A"),
+                     [("A",set_sort)])
+
+
+val Thm_2_7_assoc = proved_th $
 e0
-(strip_assume_tac AX0 >> strip_assume_tac lemma (* >>
- qspecl_then [‘A’,‘A’,‘R’] strip_assume_tac AX2 *))
+(cheat)
 (form_goal
-“?Empty. !a:mem(Empty).F”)
- parse_term_with_cont ct "R"
+“!A B phi:A->B C psi:B->C D chi:C->D. (chi o psi) o phi = chi o psi o phi”)
+
+
+val Thm_2_7_id = proved_th $
+e0
+(cheat)
+(form_goal
+“!A B phi:A->B. phi o id(A) = phi & id(B) o phi = phi”)
+
+val Thm_2_7_bij = proved_th $
+e0
+(cheat)
+(form_goal
+ “!A B phi:A->B.isBij(phi) <=> ?psi:B->A. psi o phi = id(A) & phi o psi = id(B)”)
+
+(*val _ = new_fun "*" (set_sort,[("A",set_sort),("B",set_sort)]) *)
+(*
+For sets A and B, let ⊤:A↬B denote the relation such that ⊤(x,y) holds always. A tabulation of ⊤ is denoted A×B; it is a set equipped with functions p:A×B→A and q:A×B→B such that for any x∈A and y∈B, there exists a unique z∈A×B with p(z)=x and q(z)=y. It is called the cartesian product of A and B.
+Theorem 2.8. For any sets A and B, A×B is a product of A and B in the category Set, and a coproduct in the category Rel.
 *)
 
-“Holds(R:rel(A,B),x:mem(A),y:mem(B)) & a:mem(A) = a”
+val T_ex = proved_th $
+e0
+cheat
+(form_goal
+“!A B. ?T0:A->B. !a b. Holds(T0,a,b)”)
+
+val Cross_ex = proved_th $
+e0
+(cheat)
+(form_goal
+ “!A B. ?AxB pi1:AxB ->A pi2:AxB ->B.
+  (!x:mem(A) y:mem(B). ?r:mem(AxB).Eval(pi1,r) = x & Eval(pi2,r) = y) &
+   !r s. Eval(pi1,r) = Eval(pi1,s) & Eval(pi2,r) = Eval(pi2,s)
+  ”)
+
+val Cross_def = 
+    Cross_ex |> spec_all |> eqT_intro 
+             |> iffRL |> ex2fsym "*" ["A","B"] 
+             |> C mp (trueI []) |> gen_all
+
+val pi1_def = 
+   Cross_def |> spec_all |> eqT_intro 
+             |> iffRL |> ex2fsym "pi1" ["A","B"] 
+             |> C mp (trueI []) |> gen_all
+
+val pi2_def = 
+   pi1_def |> spec_all |> eqT_intro 
+             |> iffRL |> ex2fsym "pi2" ["A","B"] 
+             |> C mp (trueI []) |> gen_all
+
+val _ = new_fun "Top" (rel_sort (mk_set "A") (mk_set "B"),
+                       [("A",set_sort),("B",set_sort)])
+
+val _ = new_pred "isSetPr" [("p1",rel_sort (mk_set "AxB") (mk_set "A")),
+                            ("p2",rel_sort (mk_set "AxB") (mk_set "B"))]
+
+val SetPr_def = new_ax
+“!A B AxB p1:AxB->A p2:AxB->B. 
+isSetPr(p1,p2) <=>
+!X f:X->A g:X->B.isFun(f) & isFun(g) ==> ?!fg: X->AxB.p1 o fg = f & p2 o fg = g”
 
 
-(*how to implement
-Axiom 1 (Relational comprehension): For any two sets A and B, and any property P that can obtain of an element of A and an element of B, there exists a unique relation φ:A↬B such that φ(x,y) if and only if P obtains of x and y.
+
+val _ = new_pred "isRelcP" [("i1",rel_sort (mk_set "A") (mk_set "AuB")),
+                            ("i2",rel_sort (mk_set "B") (mk_set "AuB"))]
+
+val RelcoPr_def = new_ax
+“!A B AuB i1:A->AuB i2:B->AuB. 
+isRelcP(i1,i2) <=>
+!X f:A->X g:B->X.?!fg:AuB ->X. fg o i1 = f & fg o i2 = g”
+
+val Thm_2_8_SetPr = proved_th $
+e0
+(cheat)
+(form_goal
+“!A B. isSetPr(pi1(A,B),pi2(A,B))”)
+
+val SPa_ex =
+let val th0 = rewr_rule[SetPr_def] Thm_2_8_SetPr
+    val f = th0 |> spec_all |> concl |> snd o dest_imp
+    val th1 = uex_ex f
+    val th0' = strip_all_and_imp th0
+    val th2 = mp th1 th0' 
+in disch_all th2 |> gen_all
+end 
+
+val SPa_def = 
+    SPa_ex |> spec_all |> ex2fsym "SPa" ["f","g"] 
+ 
+
+val RelcP_ex = proved_th $
+e0
+(cheat)
+(form_goal
+“!A B. ?i1:A->A * B i2:B->A * B.
+ !a b ab. Holds(i1,a,ab) <=> a = Eval(pi1(A,B),ab) & 
+          Holds(i2,b,ab) <=> b = Eval(pi2(A,B),ab)”)
+
+val tau1_def = 
+    RelcP_ex |> spec_all |> eqT_intro 
+             |> iffRL |> ex2fsym "tau1" ["A","B"] 
+             |> C mp (trueI []) |> gen_all
+
+val tau2_def = 
+    tau1_def |> spec_all |> eqT_intro 
+             |> iffRL |> ex2fsym "tau2" ["A","B"] 
+             |> C mp (trueI []) |> gen_all
+
+val Thm_2_8_RelcP = proved_th $
+e0
+(cheat)
+(form_goal
+“!A B. isRelcP(tau1(A,B),tau2(A,B))”)
+
+(*
+Theorem 2.9. The category Set has finite limits.
+
+Proof. It remains to construct the equalizer of two functions f,g:A→B. Let S be the subset of A so that x∈S just when f(x)=g(x); then |S|→A is easily shown to be an equalizer of f and g.  ▮
 *)
+
+val _ = new_pred "SetEz" [("f",rel_sort (mk_set "A") (mk_set "B")),
+                           ("g",rel_sort (mk_set "A") (mk_set "B")),
+                           ("e",rel_sort (mk_set "E") (mk_set "A"))]
+
+(*thesetting is considering two categories at the same time, any thing to do for that?, below is ugly, have not tested if some of e or x0 is a function can be proved rather than stated*)
+
+val SetEz_def = new_ax
+“!A B f:A->B g:A->B E e:E->A. SetEz(f,g,e) <=>
+ isFun(f) & isFun(g) & isFun(e) & !X x:X->A.isFun(x) & f o x = g o x ==> ?!x0:X->E. isFun(x0) & x = e o x0”
+
+val Thm_2_9_Eqlz = proved_th $
+e0
+(cheat)
+(form_goal
+“!A B f:A->B g:A->B.isFun(f) & isFun(g) ==> ?E e:E->A.SetEz(f,g,e)”)
+
+(*
+
+Theorem 2.10. For any function f:A→B we have f=me, where m:im(f)↪B is an injection and e:A↠im(f) is a surjection. A set im(f) equipped with such m and e is unique up to bijection and is called the image of f.
+
+
+*)
+
+val Thm_2_10 = proved_th $
+e0
+(cheat)
+(form_goal
+“!A B f:A->B. isFun(f) ==> ?M e:A->M m:M->B. f = m o e & isInj(e) & isSurj(m)”)
+
+
+(*2.11 left to tomorrow...*)
+
+(*
+Axiom 3 (power sets): For any set A, there exists a set PA and a relation ϵ:A↬PA such that for any subset S of A, there exists a unique s∈PA with the property that for any x∈A, we have x∈S iff ϵ(x,s).
+*)
+
+(*val _ = new_fun "Pow" (set_sort,[("A",set_sort)]) *)
+
+val AX3 = new_ax 
+“!A. ?PA e:A->PA. !S0:1->A.?!s:mem(PA). !x:mem(A). Holds(S0,star,x) <=> 
+ Holds(e,x,s)”
+
+(*
+Theorem 2.12. For any relation R:B↬A, there exists a unique function fR:B→PA such that R(y,x) if and only if ϵ(x,fR(y)). It follows that Set is a topos (and Rel is a power allegory).
+*)
+
+val Pow_def = 
+    AX3 |> spec_all |> eqT_intro 
+        |> iffRL |> ex2fsym "Pow" ["A"] 
+        |> C mp (trueI []) |> gen_all
+
+
+val eps_def = 
+    Pow_def |> spec_all |> eqT_intro 
+            |> iffRL |> ex2fsym "eps" ["A"] 
+            |> C mp (trueI []) |> gen_all
+
+
+(*filter cont correct?*)
+
+(*want subset notation, give a ref to tokenizer?*)
+
+(*base change*)
+
+val BC_ex = proved_th $
+e0
+(cheat)
+(form_goal
+“!Z Y f:Z->Y. ?BCf:Pow(Y) -> Pow(Z). 
+ !ys:mem(Pow(Y)) zs:mem(Pow(Z)). Holds(BCf,ys,zs) <=>
+ !z:mem(Z). Holds(eps(Z),z,zs) ==> Holds(eps(Y),Eval(f,z),ys)”)
+
+val BC_def = 
+    BC_ex |> spec_all |> eqT_intro 
+          |> iffRL |> ex2fsym "BC" ["f"] 
+          |> C mp (trueI []) |> gen_all
+
+(*TODO: show BC is a functor Pow(B) ->Pow (A)*)
+val InPow_def = 
+ let val f = concl $ spec_all eps_def
+     val uth = uex_def f
+     val th0 = rewr_rule[uth] eps_def
+     val th1 = spec_all th0
+ in th1 |>  eqT_intro |> iffRL |> ex2fsym "InPow" ["S0"] 
+        |> C mp (trueI []) |> gen_all
+ end
+
+
+(*sub*)
+fun Pow A = mk_fun "Pow" [A]
+
+(*poset order of P(A)*)
+val _ = new_pred "PO"[("S1",mem_sort (Pow (mk_set "A"))),
+                       ("S2",mem_sort (Pow (mk_set "A")))]
+
+val PO_def = new_ax
+“!A S1:mem(Pow(A)) S2:mem(Pow(A)).
+ PO(S1,S2) <=> !a. Holds(eps(A),a,S1) ==> Holds(eps(A),a,S1)”
+
+val Thm_2_11_SEx_ex = proved_th $
+e0
+cheat
+(form_goal
+ “!Z Y f:Z->Y. ?Ef:Pow(Z)-> Pow(Y). isFun(Ef) &
+  !zs:mem(Pow(Z)) ys:mem(Pow(Y)). PO(Eval(Ef,zs),ys) <=> PO(zs,Eval(BC(f),ys))”)
+
+
+val Thm_2_11_SAll_ex = proved_th $
+e0
+cheat
+(form_goal
+ “!Z Y f:Z->Y. ?Af:Pow(Z)-> Pow(Y). isFun(Af) &
+  !ys:mem(Pow(Y)) zs:mem(Pow(Z)). PO(Eval(BC(f),ys),zs) <=> PO(ys,Eval(Af,zs))”)
+
+(*
+Definition 2.1. An allegory is a locally posetal 2-category A equipped with an involution (−)o:Aop→A which is the identity on objects, such that
+
+the involution is order preserving and distributes over composition, i.e. (ψϕ)o=ϕoψo,
+each hom-poset A(x,y) has binary meets, and
+
+*)
+
+val _ = new_fun "OP" (rel_sort (mk_set "A") (mk_set "B"),
+                      [("R",rel_sort (mk_set "A") (mk_set "B"))])
+
+val OP_ex = proved_th $
+e0
+cheat
+(form_goal
+“!A B R:A->B. ?R':B->A. !a b. Holds(R,a,b) <=> Holds(R',b,a)”)
+
+val OP_def = 
+    OP_ex |> spec_all |> eqT_intro |> iffRL |> ex2fsym "OP" ["R"] 
+          |> C mp (trueI []) |> gen_all
+
+val OP_DISTR = proved_th $
+e0
+cheat
+(form_goal
+“!A B phi:A->B C psi:B->C. OP(psi o phi) = OP(phi) o OP(psi)”)
+
+(*
+If x and y are elements of a poset, then their meet is an element x∧y of the poset such that:
+
+x∧y≤x and x∧y≤y;
+if a≤x and a≤y, then a≤x∧y.
+*)
+
+val _ = new_pred "Sub" [("R1",rel_sort (mk_set "A") (mk_set "B")),
+                        ("R2",rel_sort (mk_set "A") (mk_set "B"))]
+
+val Sub_def = new_ax 
+“!A B R1:A->B R2. Sub(R1,R2) <=> !a b. Holds(R1,a,b) ==> Holds(R2,a,b)”
+
+
+val Meet_ex = proved_th $
+e0
+(cheat)
+(form_goal 
+ “!A B R1:A->B R2:A->B. ?M:A->B. !a b. Holds(M,a,b) <=> Holds(R1,a,b) & Holds(R2,a,b)”)
+
+
+val Meet_def = Meet_ex |> spec_all |> eqT_intro |> iffRL 
+                       |> ex2fsym "Meet" ["R1","R2"] 
+                       |> C mp (trueI []) |> gen_all
+
+val Meet_property = proved_th $
+e0
+(cheat)
+(form_goal
+“!A B R1:A->B R2:A->B. Sub(Meet(R1,R2),R1) & Sub(Meet(R1,R2),R2) &
+ !R0. Sub(R0,R1) & Sub(R0,R2) ==> Sub(R0,Meet(R1,R2))”)
+
+
+val Join_ex = proved_th $
+e0
+(cheat)
+(form_goal 
+ “!A B R1:A->B R2:A->B. ?J:A->B. !a b. Holds(J,a,b) <=> Holds(R1,a,b) | Holds(R2,a,b)”)
+
+
+val Join_def = Join_ex |> spec_all |> eqT_intro |> iffRL 
+                       |> ex2fsym "Join" ["R1","R2"] 
+                       |> C mp (trueI []) |> gen_all
+
+(*
+If x and y are elements of a poset P, then their join (or supremum, abbreviate sup, or least upper bound, abbreviated lub), is an element x∨y of the poset such that:
+
+x≤x∨y and y≤x∨y;
+if x≤a and y≤a, then x∨y≤a.
+
+*)
+
+val Join_property = proved_th $
+e0
+(cheat)
+(form_goal
+“!A B R1:A->B R2:A->B. Sub(R1,Join(R1,R2)) & Sub(R2,Join(R1,R2)) &
+ !R0. Sub(R0,R1) & Sub(R0,R2) ==> Sub(Join(R1,R2),R0)”)
+
+(*the modular law holds: for ϕ:x→y, ψ:y→z, and χ:x→z, we have ψϕ∩χ≤ψ(ϕ∩ψoχ).*)
+
+val MODULAR_LAW = proved_th $
+e0
+(cheat)
+(form_goal
+ “!x y phi:x->y z psi:y->z chi:x->z. 
+  Sub(Meet(psi o phi,chi),psi o Meet(phi,OP(psi) o chi))”)
+
+(*
+A union allegory Is an allegory whose hom-posets have finite joins that are preserved by composition. Thus a union allegory is locally a lattice. If additionally it is locally a distributive lattice, it is called a distributive allegory.
+*)
+
+val left_o_pres_Join = proved_th $
+e0
+cheat
+(form_goal
+ “!A B R1:A->B R2:A->B R:B->C. R o Join(R1,R2) = Join(R o R1, R o R2)”)
+
+
+val right_o_pres_Join = proved_th $
+e0
+cheat
+(form_goal
+ “!A B R1:A->B R2:A->B R:C->A. Join(R1,R2) o R = Join(R1 o R, R2 o R)”)
+
+
+(*
+A division allegory is a distributive allegory in which composition on one (and therefore the other) side has a right adjoint (left or right division). That is: given r:A→B and s:A→C, there exists s/r:B→C such that
+
+t≤s/r∈hom(B,C)⇔t∘r≤s∈hom(A,C)
+*)
+
+val Div_ex = proved_th $
+e0
+cheat
+(form_goal
+ “!A B r:A->B C s:A->C. ?sdr:B->C. 
+  !t.Sub(t,sdr) <=> Sub(t o r,s)”)
+
+val Thm_2_12 = proved_th $
+e0
+(cheat)
+(form_goal
+“!B A R:B->A.?!fR:B->Pow(A).isFun(fR) & !y x.(Holds(R,y,x) <=> Holds(eps(A),x,Eval(fR,y)))”)
+
+(*
+Theorem 2.13. For any two sets A and B, there exists a set BA and a function ev:BA×A→B such that for any function f:A→B there exists a unique element sf∈BA such that ev(sf,a)=f(a) for all a∈A. It follows that Set is a cartesian closed category.
+*)
+
+
+val Thm_2_3_5 = proved_th $
+e0
+cheat
+(form_goal
+ “!A a:mem(A). ?!R:1->A. isFun(R) & Eval(R,star) = a”)
+
+(*mem as fun*)
+val MF_def =
+let val f = concl $ spec_all Thm_2_3_5
+    val uth = uex_def f
+    val th = dimp_mp_l2r (spec_all Thm_2_3_5) uth
+in
+th |> eqT_intro |> iffRL |> ex2fsym "MF"["a"]
+   |> C mp (trueI []) |> gen_all
+end
+
+(*
+val mem_pair = proved_th $
+e0
+()
+(form_goal
+“!A B a:mem(A) b:mem(B).Eval(Spa(MF(a),MF(b)),star)”)
+*)
+
+val Thm_2_13 = proved_th $
+e0
+(cheat)
+(form_goal
+“!A B.?A2B ev:A2B * A ->B. isFun(ev) & 
+ !f:A->B.isFun(f) ==> ?!sf:mem(A2B).!a:mem(A).Eval(ev,Eval(SPa(MF(sf),MF(a)),star)) = Eval(f,a)”)
+
+(*
+
+Theorem 2.14. If R is an equivalence relation on A, then there is a surjective function q:A↠B such that R(x,y) holds iff q(x)=q(y).
+*)
+val _ = new_pred "ER" [("R",rel_sort (mk_set "A") (mk_set "A"))]
+
+val _ = new_pred "Refl" [("R",rel_sort (mk_set "A") (mk_set "A"))]
+
+val Refl_def = new_ax
+ “!A R:A->A. Refl(R) <=> !a. Holds(R,a,a)”
+val _ = new_pred "Sym" [("R",rel_sort (mk_set "A") (mk_set "A"))]
+
+val Sym_def = new_ax
+ “!A R:A->A. Sym(R) <=> !a1 a2. Holds(R,a1,a2) ==> Holds(R,a2,a1)”
+
+val _ = new_pred "Trans" [("R",rel_sort (mk_set "A") (mk_set "A"))]
+
+val Trans_def = new_ax
+ “!A R:A->A. Trans(R) <=> !a1 a2 a3. Holds(R,a1,a2) & Holds(R,a2,a3) ==> Holds(R,a1,a3)”
+
+val ER_def = new_ax
+“!A R:A->A. ER(R) <=> Refl(R) & Sym(R) & Trans(R)”
+
+val Thm_2_14 = proved_th $
+e0
+(cheat)
+(form_goal
+“!A R:A->A. ER(R) ==> ?B q:A->B. isSurj(q) & !x y.Holds(R,x,y) <=> Eval(q,x) = Eval(q,y)”)
+
+(*
+Axiom 4 (Infinity): There exists a set N, containing an element o, and a function s:N→N such that s(n)≠o for any n∈N and s(n)=s(m) only if n=m for any n,m∈N.
+*)
+
+val AX4 = new_ax
+“?N z:mem(N) s:N->N. isFun(s) & !n:mem(N). ~(Eval(s,n) = z) & 
+ !n m. Eval(s,n) = Eval(s,m) <=> n = m”
+
+(*Axiom 5 (Collection): For any set A and any property P which can obtain of an element of A and a set, there exists a set B, function p:B→A, and a B-indexed family of sets M:B↬Y such that (1) P(p(b),Mb) holds for any b∈B, and (2) for any a∈A, if there exists a set X with P(a,X), then a∈im(p).
+
+can not have im(p) as function, since then we have func that takes ar into sets
+*)
+
+fun Eval f e = mk_fun "Eval" [f,e] 
+
+val P = “?f:A-> X. Eval(f,a) = x0”
+val (n,s) = ("a", mem_sort (mk_set "A"))
+val ns = (n,s)
+val (sn,ss) = ("X",set_sort)
+val S0 = (sn,ss)
+ 
+fun AX5 P (ns as (n,s)) (S0 as(sn,ss)) = 
+    let val (sortname,A0) = dest_sort s
+        val A = if sortname = "mem" then hd A0
+                else raise ERR ("first input not a member.",[],[mk_var ns],[])
+        val ct = fvf P
+        val B = pvariantt ct (mk_set "B")
+        val (Bn,Bs) = dest_var B
+        val p = pvariantt ct (mk_rel "p" B (mk_set "A"))
+        val (pn,ps) = dest_var p
+        val Y = pvariantt ct (mk_set "Y")
+        val (Yn,Ys) = dest_var Y
+        val M = pvariantt ct (mk_rel "M" B Y)
+        val (Mn,Ms) = dest_var M
+        val b = pvariantt ct (mk_mem "b" B)
+        val (bn,bs) = dest_var b
+        val substed = substf (S0,Eval M b) (substf (ns,Eval p b) P)
+        val cj1 = mk_forall bn bs substed
+        val X = pvariantt ct (mk_set "X")
+        val a = pvariantt ct (mk_mem "a" A)
+        val (aan,aas) = dest_var a
+        val substed' = substf (S0,X) (substf (ns,a) P)
+        val b0 = pvariantt ct (mk_mem "b0" B)
+        val (b0n,b0s) = dest_var b0
+        val concl2 = mk_exists b0n b0s (mk_eq (Eval p b0) a)
+        val cj2 = mk_forall aan aas (mk_imp substed' concl2)
+        val cjs = mk_conj cj1 cj2
+        val f = mk_exists Bn Bs $ mk_exists pn ps $
+                          mk_exists Yn Ys $ mk_exists Mn Ms cjs
+    in mk_thm(fvf f,[],f) 
+    end
+
+
